jar2bpl_test/regression/test_output/java_input.bpl
@@ -9,16 +9,14 @@ type intArrHeap_type = [ref][int]int;
 const unique $type : Field javaType;
 const unique $alloc : Field bool;
 const unique $null : ref;
-const { :sourceloc "Object.java",-1,-1,-1,-1 } unique java.lang.Object : javaType extends  complete;
-const { :sourceloc "FalsePositives04.java",-1,-1,-1,-1 } unique FalsePositives04 : javaType extends  unique java.lang.Object complete;
-const { :sourceloc "Serializable.java",-1,-1,-1,-1 } unique java.io.Serializable : javaType extends  unique java.lang.Object complete;
-const { :sourceloc "Throwable.java",-1,-1,-1,-1 } unique java.lang.Throwable : javaType extends  unique java.io.Serializable, unique java.lang.Object complete;
-const { :sourceloc "Exception.java",-1,-1,-1,-1 } unique java.lang.Exception : javaType extends  unique java.lang.Throwable complete;
-const { :sourceloc "RuntimeException.java",-1,-1,-1,-1 } unique java.lang.RuntimeException : javaType extends  unique java.lang.Exception complete;
-const { :sourceloc "NullPointerException.java",-1,-1,-1,-1 } unique java.lang.NullPointerException : javaType extends  unique java.lang.RuntimeException complete;
-const { :sourceloc "Comparable.java",-1,-1,-1,-1 } unique java.lang.Comparable : javaType extends  unique java.lang.Object complete;
-const { :sourceloc "CharSequence.java",-1,-1,-1,-1 } unique java.lang.CharSequence : javaType extends  unique java.lang.Object complete;
-const { :sourceloc "String.java",-1,-1,-1,-1 } unique java.lang.String : javaType extends  unique java.io.Serializable, unique java.lang.CharSequence, unique java.lang.Comparable, unique java.lang.Object complete;
+const { :sourceloc "/Users/schaef/git/jar2bpl/jar2bpl_test/regression/false_positives/fp06/FalsePositives06.javaFalsePositives06.java",-1,-1,-1,-1 } unique java.lang.Object : javaType extends  complete;
+const { :sourceloc "/Users/schaef/git/jar2bpl/jar2bpl_test/regression/false_positives/fp06/FalsePositives06.javaFalsePositives06.java",-1,-1,-1,-1 } unique java.io.Serializable : javaType extends  unique java.lang.Object complete;
+const { :sourceloc "/Users/schaef/git/jar2bpl/jar2bpl_test/regression/false_positives/fp06/FalsePositives06.javaFalsePositives06.java",-1,-1,-1,-1 } unique FalsePositives06$FilterMap : javaType extends  unique java.io.Serializable, unique java.lang.Object complete;
+const { :sourceloc "/Users/schaef/git/jar2bpl/jar2bpl_test/regression/false_positives/fp06/FalsePositives06.javaFalsePositives06.java",-1,-1,-1,-1 } unique FalsePositives06 : javaType extends  unique java.lang.Object complete;
+const { :sourceloc "/Users/schaef/git/jar2bpl/jar2bpl_test/regression/false_positives/fp06/FalsePositives06.javaFalsePositives06.java",-1,-1,-1,-1 } unique FalsePositives06$ContextFilterMaps : javaType extends  unique java.lang.Object complete;
+const { :sourceloc "/Users/schaef/git/jar2bpl/jar2bpl_test/regression/false_positives/fp06/FalsePositives06.javaFalsePositives06.java",-1,-1,-1,-1 } unique java.lang.Throwable : javaType extends  unique java.io.Serializable, unique java.lang.Object complete;
+const { :sourceloc "/Users/schaef/git/jar2bpl/jar2bpl_test/regression/false_positives/fp06/FalsePositives06.javaFalsePositives06.java",-1,-1,-1,-1 } unique java.lang.Exception : javaType extends  unique java.lang.Throwable complete;
+const { :sourceloc "/Users/schaef/git/jar2bpl/jar2bpl_test/regression/false_positives/fp06/FalsePositives06.javaFalsePositives06.java",-1,-1,-1,-1 } unique java.lang.RuntimeException : javaType extends  unique java.lang.Exception complete;
 var $heap : $heap_type;
 var $intArrayType : javaType;
 var $charArrayType : javaType;
@@ -31,7 +29,10 @@ var $boolArrHeap : boolArrHeap_type;
 var $refArrHeap : refArrHeap_type;
 var $realArrHeap : realArrHeap_type;
 var $intArrHeap : intArrHeap_type;
-var java.lang.Object$FalsePositives04$first234 : Field ref;
+var FalsePositives06$FalsePositives06$FilterMap$this$0236 : Field ref;
+var java.lang.Object$FalsePositives06$ContextFilterMaps$lock234 : Field ref;
+var FalsePositives06$FilterMap$lp$$rp$$FalsePositives06$ContextFilterMaps$array235 : Field ref;
+var int$FalsePositives06$ContextFilterMaps$insertPoint0 : Field int;
 function $arrayType(t:javaType) returns ($ret:javaType);
 function $intToReal(x:int) returns ($ret:real);
 function $intToBool(x:int) returns ($ret:bool) { (if x == 0 then false else true) }
@@ -50,126 +51,131 @@ function $shrInt(x:int, y:int) returns ($ret:int);
 axiom (forall t : javaType :: $heap[$null,$type] <: t);
 procedure $new(obj_type:javaType) returns ($obj:ref);    ensures $heap[$obj,$type] == obj_type;    requires $heap[$obj,$alloc] == false;        ensures $obj != $null;    ensures $heap[$obj,$alloc] == true;
 
-procedure java.lang.Object$java.lang.Object$clone$43($this:ref) returns ($other:ref);        ensures $other != $null;    ensures $heap[$other,$alloc] == true;    ensures $heap[$other,$type] == $heap[$this,$type];
+procedure java.lang.Object$java.lang.Object$clone$43($this:ref) returns ($other:ref);        ensures $heap[$other,$alloc] == true;    ensures $other != $null;    ensures $heap[$other,$type] == $heap[$this,$type];
 
 procedure int$java.lang.String$compareTo$87($this:ref, $other:ref) returns ($return:int);    
 
-procedure java.lang.Object$FalsePositives04$peekFirst$1890($this:ref) returns ($return:ref, $exception:ref);    modifies $heap;
-
-procedure java.lang.Object$FalsePositives04$foo$1889($this:ref) returns ($return:ref, $exception:ref);    modifies $heap;
-
-procedure java.lang.String$java.lang.Object$toString$44($this:ref) returns ($return:ref, $exception:ref);    
-
-procedure void$FalsePositives04$$la$init$ra$$1891($this:ref) returns ($exception:ref);    
+procedure void$FalsePositives06$FilterMap$$la$init$ra$$1889($this:ref, $in_parameter__0:ref) returns ($exception:ref);    modifies $heap;
 
 procedure void$java.lang.Object$$la$init$ra$$38($this:ref) returns ($exception:ref);    
 
-implementation java.lang.Object$FalsePositives04$peekFirst$1890($this:ref) returns ($return:ref, $exception:ref){
+procedure FalsePositives06$FilterMap$lp$$rp$$FalsePositives06$ContextFilterMaps$asArray$1890($this:ref) returns ($return:ref, $exception:ref);    
+
+procedure void$FalsePositives06$ContextFilterMaps$$la$init$ra$$1891($this:ref) returns ($exception:ref);    modifies $heap, $arrSizeHeap;
+
+procedure void$FalsePositives06$$la$init$ra$$1892($this:ref) returns ($exception:ref);    
+
+implementation void$FalsePositives06$FilterMap$$la$init$ra$$1889($this:ref, $in_parameter__0:ref) returns ($exception:ref){
     
-var temp$24 : ref;    
 var this1 : ref;    
-var temp$35 : ref;    
-var temp$13 : ref;    
-var temp$68 : ref;    
-var temp$57 : ref;    
-var temp$79 : ref;    
-var temp$02 : ref;    
-var temp$46 : ref;
-    assume $this != $null;
-    assume $heap[$return,$type] <: java.lang.Object;
-    assert { :sourceloc "FalsePositives04.java",8,5,17,5 } true;
+var temp$02 : ref;
+    assume { :sourceloc "/Users/schaef/git/jar2bpl/jar2bpl_test/regression/false_positives/fp06/FalsePositives06.javaFalsePositives06.java",-1,-1,-1,-1 } $this != $null;
+    assume $heap[$in_parameter__0,$type] <: FalsePositives06;
+    assert { :sourceloc "/Users/schaef/git/jar2bpl/jar2bpl_test/regression/false_positives/fp06/FalsePositives06.javaFalsePositives06.java",8,-1,-1,-1 } true;
     this1 := $this;
-  block1:
-    assert { :sourceloc "FalsePositives04.java",8,5,17,5 } true;
-    assert { :sourceloc "FalsePositives04.java",10,18,10,22 } true;
-    call temp$02, $exception := java.lang.Object$FalsePositives04$foo$1889(this1);
-    if ($exception != $null && $heap[$exception,$type] <: java.lang.Throwable) {
-        goto block2;
-    }
-    assert { :sourceloc "FalsePositives04.java",10,10,10,14 } true;
-    $heap := $heap[this1,java.lang.Object$FalsePositives04$first234 := temp$02];
-    assert { :sourceloc "FalsePositives04.java",11,20,11,24 } true;
-    temp$13 := $heap[this1,java.lang.Object$FalsePositives04$first234];
-    assert { :sourceloc "FalsePositives04.java",11,20,11,24 } true;
-    if (temp$13 != $null) {
-        assert { :sourceloc "FalsePositives04.java",11,20,11,24 } true;
-    } else {
-        assert { :noverify } true;
-        call $exception := $new(java.lang.NullPointerException);
-        goto block2;
-    }
-    call temp$24, $exception := java.lang.String$java.lang.Object$toString$44(temp$13);
-    if ($exception != $null && $heap[$exception,$type] <: java.lang.Throwable) {
-        goto block2;
-    }
-  block3:
-    assert { :sourceloc "FalsePositives04.java",11,20,11,24 } true;
-    assert { :sourceloc "FalsePositives04.java",13,14,13,18 } { :clone } true;
-    assert { :sourceloc "FalsePositives04.java",13,14,13,18 } { :clone } this1 != $null;
-    temp$35 := $heap[this1,java.lang.Object$FalsePositives04$first234];
-    assert { :sourceloc "FalsePositives04.java",13,14,13,18 } { :clone } true;
-    if (temp$35 == $null) {
-        assert { :sourceloc "FalsePositives04.java",13,14,13,18 } { :clone } true;
-        goto block4;
-    } else {
-        assert { :sourceloc "FalsePositives04.java",13,14,13,18 } { :clone } true;
-    }
-    assert { :sourceloc "FalsePositives04.java",13,14,13,18 } { :clone } true;
-    goto block5;
-  block4:
-    assert { :sourceloc "FalsePositives04.java",13,14,13,18 } { :clone } true;
-    assert { :sourceloc "FalsePositives04.java",13,14,13,18 } { :clone } true;
-    temp$46 := $null;
-    assert { :sourceloc "FalsePositives04.java",14,11,14,22 } true;
-    $return := temp$46;
-    return;
-  block5:
-    assert { :sourceloc "FalsePositives04.java",14,11,14,22 } true;
-    assert { :sourceloc "FalsePositives04.java",11,13,11,36 } true;
-    $return := temp$24;
-    return;
-  block2:
-    assert { :sourceloc "FalsePositives04.java",11,13,11,36 } true;
-    assert { :sourceloc "FalsePositives04.java",9,9,16,9 } true;
-    assert { :sourceloc "FalsePositives04.java",9,9,16,9 } $exception != $null;
-    assume $heap[$exception,$type] <: java.lang.Throwable;
-    temp$57 := $exception;
-    assert { :sourceloc "FalsePositives04.java",13,14,13,18 } { :clone } true;
-    assert { :sourceloc "FalsePositives04.java",13,14,13,18 } { :clone } this1 != $null;
-    temp$68 := $heap[this1,java.lang.Object$FalsePositives04$first234];
-    assert { :sourceloc "FalsePositives04.java",13,14,13,18 } { :clone } true;
-    if (temp$68 == $null) {
-        assert { :sourceloc "FalsePositives04.java",13,14,13,18 } { :clone } true;
-        goto block6;
-    } else {
-        assert { :sourceloc "FalsePositives04.java",13,14,13,18 } { :clone } true;
-    }
-    assert { :sourceloc "FalsePositives04.java",13,14,13,18 } { :clone } true;
-    goto block7;
-  block6:
-    assert { :sourceloc "FalsePositives04.java",13,14,13,18 } { :clone } true;
-    assert { :sourceloc "FalsePositives04.java",13,14,13,18 } { :clone } true;
-    temp$79 := $null;
-    assert { :sourceloc "FalsePositives04.java",14,11,14,22 } true;
-    $return := temp$79;
-    return;
-  block7:
-    assert { :sourceloc "FalsePositives04.java",14,11,14,22 } true;
-    assert { :sourceloc "FalsePositives04.java",14,11,14,22 } true;
-    $exception := temp$57;
+    assert { :sourceloc "/Users/schaef/git/jar2bpl/jar2bpl_test/regression/false_positives/fp06/FalsePositives06.javaFalsePositives06.java",8,-1,-1,-1 } true;
+    temp$02 := $in_parameter__0;
+    assert { :sourceloc "/Users/schaef/git/jar2bpl/jar2bpl_test/regression/false_positives/fp06/FalsePositives06.javaFalsePositives06.java",8,-1,-1,-1 } true;
+    call $exception := void$java.lang.Object$$la$init$ra$$38(this1);
+    assert { :sourceloc "/Users/schaef/git/jar2bpl/jar2bpl_test/regression/false_positives/fp06/FalsePositives06.javaFalsePositives06.java",8,-1,-1,-1 } true;
+    assert { :sourceloc "/Users/schaef/git/jar2bpl/jar2bpl_test/regression/false_positives/fp06/FalsePositives06.javaFalsePositives06.java",8,-1,-1,-1 } this1 != $null;
+    $heap := $heap[this1,FalsePositives06$FalsePositives06$FilterMap$this$0236 := temp$02];
+    assert { :sourceloc "/Users/schaef/git/jar2bpl/jar2bpl_test/regression/false_positives/fp06/FalsePositives06.javaFalsePositives06.java",8,-1,-1,-1 } true;
     return;
 }
 
 
-implementation void$FalsePositives04$$la$init$ra$$1891($this:ref) returns ($exception:ref){
+implementation FalsePositives06$FilterMap$lp$$rp$$FalsePositives06$ContextFilterMaps$asArray$1890($this:ref) returns ($return:ref, $exception:ref){
     
-var this10 : ref;
-    assume $this != $null;
-    assert { :sourceloc "FalsePositives04",3,-1,-1,-1 } true;
-    this10 := $this;
-    assert { :sourceloc "FalsePositives04",3,-1,-1,-1 } true;
-    call $exception := void$java.lang.Object$$la$init$ra$$38(this10);
-    assert { :sourceloc "FalsePositives04",3,-1,-1,-1 } true;
+var temp$26 : ref;    
+var temp$15 : ref;    
+var temp$04 : ref;    
+var this3 : ref;
+    assume { :sourceloc "/Users/schaef/git/jar2bpl/jar2bpl_test/regression/false_positives/fp06/FalsePositives06.javaFalsePositives06.java",-1,-1,-1,-1 } $this != $null;
+    assert { :sourceloc "/Users/schaef/git/jar2bpl/jar2bpl_test/regression/false_positives/fp06/FalsePositives06.javaFalsePositives06.java",37,6,41,6 } true;
+    this3 := $this;
+    assert { :sourceloc "/Users/schaef/git/jar2bpl/jar2bpl_test/regression/false_positives/fp06/FalsePositives06.javaFalsePositives06.java",38,24,38,27 } true;
+    assert { :sourceloc "/Users/schaef/git/jar2bpl/jar2bpl_test/regression/false_positives/fp06/FalsePositives06.javaFalsePositives06.java",38,24,38,27 } this3 != $null;
+    temp$04 := $heap[this3,java.lang.Object$FalsePositives06$ContextFilterMaps$lock234];
+    assert { :sourceloc "/Users/schaef/git/jar2bpl/jar2bpl_test/regression/false_positives/fp06/FalsePositives06.javaFalsePositives06.java",38,24,38,27 } true;
+  block1:
+    assert { :sourceloc "/Users/schaef/git/jar2bpl/jar2bpl_test/regression/false_positives/fp06/FalsePositives06.javaFalsePositives06.java",38,24,38,27 } true;
+    assert { :sourceloc "/Users/schaef/git/jar2bpl/jar2bpl_test/regression/false_positives/fp06/FalsePositives06.javaFalsePositives06.java",39,21,39,25 } true;
+    temp$15 := $heap[this3,FalsePositives06$FilterMap$lp$$rp$$FalsePositives06$ContextFilterMaps$array235];
+    assert { :sourceloc "/Users/schaef/git/jar2bpl/jar2bpl_test/regression/false_positives/fp06/FalsePositives06.javaFalsePositives06.java",38,10,40,10 } true;
+  block3:
+    assert { :sourceloc "/Users/schaef/git/jar2bpl/jar2bpl_test/regression/false_positives/fp06/FalsePositives06.javaFalsePositives06.java",39,14,39,26 } true;
+    assert { :sourceloc "/Users/schaef/git/jar2bpl/jar2bpl_test/regression/false_positives/fp06/FalsePositives06.javaFalsePositives06.java",39,14,39,26 } true;
+    $return := temp$15;
+    return;
+  block2:
+    assert { :sourceloc "/Users/schaef/git/jar2bpl/jar2bpl_test/regression/false_positives/fp06/FalsePositives06.javaFalsePositives06.java",39,14,39,26 } true;
+    assert { :sourceloc "/Users/schaef/git/jar2bpl/jar2bpl_test/regression/false_positives/fp06/FalsePositives06.javaFalsePositives06.java",39,14,39,26 } true;
+    if ($exception != $null) {
+        assert { :sourceloc "/Users/schaef/git/jar2bpl/jar2bpl_test/regression/false_positives/fp06/FalsePositives06.javaFalsePositives06.java",39,14,39,26 } true;
+    } else {
+        assert { :noverify } true;
+        call $exception := $new(java.lang.RuntimeException);
+        goto block2;
+    }
+    assume $heap[$exception,$type] <: java.lang.Throwable;
+    temp$26 := $exception;
+    assert { :sourceloc "/Users/schaef/git/jar2bpl/jar2bpl_test/regression/false_positives/fp06/FalsePositives06.javaFalsePositives06.java",38,10,40,10 } true;
+    assert { :sourceloc "/Users/schaef/git/jar2bpl/jar2bpl_test/regression/false_positives/fp06/FalsePositives06.javaFalsePositives06.java",38,10,40,10 } true;
+    $exception := temp$26;
+    goto block2;
+  block4:
+    assert { :sourceloc "/Users/schaef/git/jar2bpl/jar2bpl_test/regression/false_positives/fp06/FalsePositives06.javaFalsePositives06.java",38,10,40,10 } true;
+}
+
+
+implementation void$FalsePositives06$ContextFilterMaps$$la$init$ra$$1891($this:ref) returns ($exception:ref){
+    
+var $fakelocal_0 : ref;    
+var $fakelocal_1 : ref;    
+var temp$210 : int;    
+var this7 : ref;    
+var temp$19 : ref;    
+var temp$08 : ref;
+    assume { :sourceloc "/Users/schaef/git/jar2bpl/jar2bpl_test/regression/false_positives/fp06/FalsePositives06.javaFalsePositives06.java",-1,-1,-1,-1 } $this != $null;
+    assert { :sourceloc "/Users/schaef/git/jar2bpl/jar2bpl_test/regression/false_positives/fp06/FalsePositives06.javaFalsePositives06.java",12,-1,-1,-1 } true;
+    this7 := $this;
+    assert { :sourceloc "/Users/schaef/git/jar2bpl/jar2bpl_test/regression/false_positives/fp06/FalsePositives06.javaFalsePositives06.java",12,-1,-1,-1 } true;
+    call $exception := void$java.lang.Object$$la$init$ra$$38(this7);
+    assert { :sourceloc "/Users/schaef/git/jar2bpl/jar2bpl_test/regression/false_positives/fp06/FalsePositives06.javaFalsePositives06.java",12,-1,-1,-1 } true;
+    call $fakelocal_0 := $new(java.lang.Object);
+    temp$08 := $fakelocal_0;
+    assert { :sourceloc "/Users/schaef/git/jar2bpl/jar2bpl_test/regression/false_positives/fp06/FalsePositives06.javaFalsePositives06.java",13,34,13,45 } true;
+    call $exception := void$java.lang.Object$$la$init$ra$$38(temp$08);
+    assert { :sourceloc "/Users/schaef/git/jar2bpl/jar2bpl_test/regression/false_positives/fp06/FalsePositives06.javaFalsePositives06.java",13,6,13,46 } true;
+    assert { :sourceloc "/Users/schaef/git/jar2bpl/jar2bpl_test/regression/false_positives/fp06/FalsePositives06.javaFalsePositives06.java",13,6,13,46 } this7 != $null;
+    $heap := $heap[this7,java.lang.Object$FalsePositives06$ContextFilterMaps$lock234 := temp$08];
+    assert { :sourceloc "/Users/schaef/git/jar2bpl/jar2bpl_test/regression/false_positives/fp06/FalsePositives06.javaFalsePositives06.java",13,6,13,46 } true;
+    call $fakelocal_1 := $new($arrayType(FalsePositives06$FilterMap));
+    $arrSizeHeap := $arrSizeHeap[$fakelocal_1 := 0];
+    temp$19 := $fakelocal_1;
+    assert { :sourceloc "/Users/schaef/git/jar2bpl/jar2bpl_test/regression/false_positives/fp06/FalsePositives06.javaFalsePositives06.java",21,6,21,50 } true;
+    assert { :sourceloc "/Users/schaef/git/jar2bpl/jar2bpl_test/regression/false_positives/fp06/FalsePositives06.javaFalsePositives06.java",21,6,21,50 } this7 != $null;
+    $heap := $heap[this7,FalsePositives06$FilterMap$lp$$rp$$FalsePositives06$ContextFilterMaps$array235 := temp$19];
+    assert { :sourceloc "/Users/schaef/git/jar2bpl/jar2bpl_test/regression/false_positives/fp06/FalsePositives06.javaFalsePositives06.java",21,6,21,50 } true;
+    temp$210 := 0;
+    assert { :sourceloc "/Users/schaef/git/jar2bpl/jar2bpl_test/regression/false_positives/fp06/FalsePositives06.javaFalsePositives06.java",32,6,32,33 } true;
+    assert { :sourceloc "/Users/schaef/git/jar2bpl/jar2bpl_test/regression/false_positives/fp06/FalsePositives06.javaFalsePositives06.java",32,6,32,33 } this7 != $null;
+    $heap := $heap[this7,int$FalsePositives06$ContextFilterMaps$insertPoint0 := temp$210];
+    assert { :sourceloc "/Users/schaef/git/jar2bpl/jar2bpl_test/regression/false_positives/fp06/FalsePositives06.javaFalsePositives06.java",32,6,32,33 } true;
+    return;
+}
+
+
+implementation void$FalsePositives06$$la$init$ra$$1892($this:ref) returns ($exception:ref){
+    
+var this11 : ref;
+    assume { :sourceloc "/Users/schaef/git/jar2bpl/jar2bpl_test/regression/false_positives/fp06/FalsePositives06.javaFalsePositives06.java",-1,-1,-1,-1 } $this != $null;
+    assert { :sourceloc "/Users/schaef/git/jar2bpl/jar2bpl_test/regression/false_positives/fp06/FalsePositives06.javaFalsePositives06.java",6,-1,-1,-1 } true;
+    this11 := $this;
+    assert { :sourceloc "/Users/schaef/git/jar2bpl/jar2bpl_test/regression/false_positives/fp06/FalsePositives06.javaFalsePositives06.java",6,-1,-1,-1 } true;
+    call $exception := void$java.lang.Object$$la$init$ra$$38(this11);
+    assert { :sourceloc "/Users/schaef/git/jar2bpl/jar2bpl_test/regression/false_positives/fp06/FalsePositives06.javaFalsePositives06.java",6,-1,-1,-1 } true;
     return;
 }
 
